# 启发性例题

## #1

求：

$$
\lim _{x \rightarrow+\infty} \sqrt{x}(\sqrt{x+2}-2 \sqrt{x+1}+\sqrt{x})
$$

原式

$$
\begin{align}
 & =\lim _{x \rightarrow+\infty} \sqrt{x}(\sqrt{x+2}-\sqrt{x+1})-\sqrt{x}(\sqrt{x+1}-\sqrt{x})
\\ & =\lim _{x \rightarrow+\infty} \frac{\sqrt{x}}{(\sqrt{x+2}+\sqrt{x+1})}-\lim _{x \rightarrow+\infty} \frac{\sqrt{x}}{(\sqrt{x+2}+\sqrt{x+1})}\\
& =\lim _{x \rightarrow+\infty} \frac{1}{(\sqrt{1+\frac{2}{x}}+\sqrt{1+\frac{1}{x}}}-\lim _{x \rightarrow+\infty} \frac{1}{(\sqrt{1+\frac{1}{x}}+\sqrt{1}}\\
&=\frac{1}{2}-\frac{1}{2}=0
\end{align}
$$

## #2

结论：

$$
\lim_{x\to x_0}u^v=e^{\lim\limits_{x\to x_0}(u-1)v}
$$

证明：

$$
\lim u^v=\lim \left\{[1+(u-1)]^\frac1{u-1}\right\}^{(u-1)v}=e^{\lim(u-1)v}
$$

## #3 柯西-施瓦尔兹不等式的运用

柯西-施瓦尔兹不等式：

$$
\left( \sum_{i=1}^{n} u_i v_i \right)^2 \leq \left( \sum_{i=1}^{n} u_i^2 \right) \left( \sum_{i=1}^{n} v_i^2 \right)
$$

已知：

$$
\sum^{n}_{k=1}a_k=1
$$

求证：

$$
\begin{align}
\sum^{n}_{k=1} (a_k+\frac{1}{a_k})^2 \ge \frac{(n^2+1)^2}{n}
\end{align}
$$

证明：

$$
\begin{align}
&\sum^{n}_{k=1} (a_k+\frac{1}{a_k})^2\\
=&\frac1n\left [\sum^{n}_{k=1} (a_k+\frac{1}{a_k})^2\times \sum^n_{k=1}1^2\right ]\\
\ge &\frac{1}{n}\left [ \sum^n_{k=1}(a_k+\frac{1}{a_k})\times1 \right ]^2\\
= &\frac{1}{n}\left [ \sum^n_{k=1}a_k+\sum^n_{k=1}a_k\times\sum^n_{k=1}\frac{1}{a_k}\right ]^2\\
\ge &\frac{1}{n}\left \{ 1+\left [ \sum^n_{k=1}(\sqrt{a_k} \times\frac{1}{\sqrt{a_k}}) \right ]^2 \right \}^2\\
=&\frac{(n^2+1)^2}{n}
\end{align}
$$

## #4

已知 $f(x)=a(x-1)^2+b(x-1)+c+\sqrt{x^2+3}$ 是 $x$ 趋于 $1$ 时 $(x-1)^2$ 的高阶无穷小，求常数 $a,b,c$。

### 法 1：配凑

设 $t=x-1,x=t+1$。

$$
\begin{align}
& \lim_{x\to1}{a(x-1)^2+b(x-1)+c-\sqrt{x^2+3}\over(x-1)^2}=0 \\
\Rightarrow & \lim_{t\to0}{at^2+bt+c-\sqrt{t^2+2t+4}\over t^2}=0 \\
\Rightarrow & \lim_{t\to0}{bt+c-\sqrt{t^2+2t+4}\over t^2}=-a \\
= & \lim_{t\to0}{(bt+c)^2-(t^2+2t+4)\over t^2(bt+c+\sqrt{t^2+2t+4})} \\
= & \lim_{t\to0}{(b^2-1)t^2+(2bc-2)t+c^2-4\over t^2(bt+c+\sqrt{t^2+2t+4})} \\
\Rightarrow & \left\{\begin{array}l
  2bc-2=0 \\
  {b^2-1\over c+2}=-a \\
  c^2-4=0
\end{array}\right.
\Rightarrow \left\{\begin{array}l
  a=\frac3{16} \\
  b=\frac12 \\
  c=2
\end{array}\right.
\end{align}
$$

### 法 2：洛必达

$$
\eqalign{
  & \mathop {\lim }\limits_{x \to 1} {{a{{(x - 1)}^2} + b(x - 1) + c - \sqrt {{x^2} + 3} } \over {{{(x - 1)}^2}}} = 0  \cr
  & {\rm{let}\:}t = x - 1,x = t + 1  \cr
  & \mathop {\lim }\limits_{t \to 0} {{a{t^2} + bt + c - \sqrt {{{(t + 1)}^2} + 3} } \over {{t^2}}} = \mathop {\lim }\limits_{t \to 0} {{a{t^2} + bt + c - \sqrt {{t^2} + 2t + 4} } \over {{t^2}}} = 0  \cr
  &  \Rightarrow \mathop {\lim }\limits_{t \to 0} a{t^2} + bt + c - \sqrt {{t^2} + 2t + 4}  = c - \sqrt 4  = 0 \Rightarrow c = 2  \cr
  &  \Rightarrow \mathop {\lim }\limits_{t \to 0} {{a{t^2} + bt + 2 - \sqrt {{t^2} + 2t + 4} } \over {{t^2}}} = a + \mathop {\lim }\limits_{t \to 0} {{bt + 2 - \sqrt {{t^2} + 2t + 4} } \over {{t^2}}} = 0  \cr
  &  \Rightarrow \mathop {\lim }\limits_{t \to 0} {{bt + 2 - \sqrt {{t^2} + 2t + 4} } \over {{t^2}}} =  - a  \cr
  & \mathop {\lim }\limits_{t \to 0} {{bt + 2 - \sqrt {{t^2} + 2t + 4} } \over {{t^2}}} = \mathop {\lim }\limits_{t \to 0} {{b - {{t + 1} \over {\sqrt {{t^2} + 2t + 4} }}} \over {2t}} =  - a  \cr
  &  \Rightarrow \mathop {\lim }\limits_{t \to 0} b - {{t + 1} \over {\sqrt {{t^2} + 2t + 4} }} = 0 \Rightarrow \mathop {\lim }\limits_{t \to 0} {{t + 1} \over {\sqrt {{t^2} + 2t + 4} }} = {1 \over {\sqrt 4 }} = {1 \over 2} = b  \cr
  &  \Rightarrow \mathop {\lim }\limits_{t \to 0} {{b - {{t + 1} \over {\sqrt {{t^2} + 2t + 4} }}} \over {2t}} = \mathop {\lim }\limits_{t \to 0}  - {3 \over 2}{({t^2} + 2t + 4)^{ - {3 \over 2}}} =  - {3 \over {2 \times 2 \times 4}} =  - {3 \over {16}} =  - a  \cr
  &  \Rightarrow a = {3 \over {16}}  \cr
  &  \Rightarrow \left\{ \matrix{
  a = {3 \over {16}}, \hfill \cr
  b = {1 \over 2}, \hfill \cr
  c = 2 \hfill \cr}  \right. \cr}
$$

注意应用洛必达的条件。

### 法 3：

$$
\begin{align}
  & \mathop {\lim }\limits_{x \to 1} {{a{{(x - 1)}^2} + b(x - 1) + c - \sqrt {{x^2} + 3} } \over {{{(x - 1)}^2}}} = 0  \\
  \Rightarrow & {\lim}\limits_{x \to 1} [{ a(x-1)^2 +b(x-1)+c- \sqrt {x^2+3} }]=0 \\
  \Rightarrow & c-\sqrt 4 = 0 \Rightarrow c=2\\
  & {\lim}\limits_{x \to 1} {a(x-1)^2+b(x-1)+c-\sqrt{x^2+3} \over (x-1)}=0 \\
  \Rightarrow &  b+{\lim}\limits_{x \to 1} {c-\sqrt{x^2+3} \over (x-1)} \Rightarrow b={1 \over 2}\\
  & {\lim }\limits_{x \to 1} {{a{{(x - 1)}^2} + b(x - 1) + c - \sqrt {{x^2} + 3} } \over {{{(x - 1)}^2}}} = 0 \\
  \Rightarrow & a+{\lim }\limits_{x \to 1} {{{ (x-1) \over 2 } + 2 - \sqrt {{x^2} + 3} } \over {{{(x - 1)}^2}}} = 0 \Rightarrow a={3 \over 16} \\
  \Rightarrow & \left\{ \matrix{
  a = {3 \over {16}}, \hfill \cr
  b = {1 \over 2}, \hfill \cr
  c = 2 \hfill \cr}  \right. \cr
\end{align}
$$

